closed -> scope.

theories/lambda_lang/well_formed.v
@@ -52,60 +52,60 @@ Fixpoint lambda_expr_well_formed prog e :=
       lambda_expr_well_formed prog e3
   end.
 
-Fixpoint lambda_expr_closed lvl e :=
+Fixpoint lambda_expr_scope scope e :=
   match e with
   | LambdaVal _ =>
       True
   | LambdaVar x =>
-      x < lvl
+      x < scope
   | LambdaLet e1 e2 =>
-      lambda_expr_closed lvl e1 ∧
-      lambda_expr_closed (S lvl) e2
+      lambda_expr_scope scope e1 ∧
+      lambda_expr_scope (S scope) e2
   | LambdaCall e1 e2 =>
-      lambda_expr_closed lvl e1 ∧
-      lambda_expr_closed lvl e2
+      lambda_expr_scope scope e1 ∧
+      lambda_expr_scope scope e2
   | LambdaUnop _ e =>
-      lambda_expr_closed lvl e
+      lambda_expr_scope scope e
   | LambdaBinop _ e1 e2 =>
-      lambda_expr_closed lvl e1 ∧
-      lambda_expr_closed lvl e2
+      lambda_expr_scope scope e1 ∧
+      lambda_expr_scope scope e2
   | LambdaBinopDet _ e1 e2 =>
-      lambda_expr_closed lvl e1 ∧
-      lambda_expr_closed lvl e2
+      lambda_expr_scope scope e1 ∧
+      lambda_expr_scope scope e2
   | LambdaIf e0 e1 e2 =>
-      lambda_expr_closed lvl e0 ∧
-      lambda_expr_closed lvl e1 ∧
-      lambda_expr_closed lvl e2
+      lambda_expr_scope scope e0 ∧
+      lambda_expr_scope scope e1 ∧
+      lambda_expr_scope scope e2
   | LambdaConstr _ e1 e2 =>
-      lambda_expr_closed lvl e1 ∧
-      lambda_expr_closed lvl e2
+      lambda_expr_scope scope e1 ∧
+      lambda_expr_scope scope e2
   | LambdaConstrDet _ e1 e2 =>
-      lambda_expr_closed lvl e1 ∧
-      lambda_expr_closed lvl e2
+      lambda_expr_scope scope e1 ∧
+      lambda_expr_scope scope e2
   | LambdaLoad e1 e2 =>
-      lambda_expr_closed lvl e1 ∧
-      lambda_expr_closed lvl e2
+      lambda_expr_scope scope e1 ∧
+      lambda_expr_scope scope e2
   | LambdaStore e1 e2 e3 =>
-      lambda_expr_closed lvl e1 ∧
-      lambda_expr_closed lvl e2 ∧
-      lambda_expr_closed lvl e3
+      lambda_expr_scope scope e1 ∧
+      lambda_expr_scope scope e2 ∧
+      lambda_expr_scope scope e3
   end.
 
 Definition lambda_program_well_formed prog :=
   map_Forall (λ _, lambda_expr_well_formed prog) prog.
 
-Definition lambda_program_closed prog :=
-  map_Forall (λ _, lambda_expr_closed 1) prog.
+Definition lambda_program_scope prog :=
+  map_Forall (λ _, lambda_expr_scope 1) prog.
 
 Definition lambda_program_valid prog :=
-  lambda_program_well_formed prog ∧ lambda_program_closed prog.
+  lambda_program_well_formed prog ∧ lambda_program_scope prog.
 
-Lemma subst_lambda_expr_closed ς1 ς2 lvl e :
-  (∀ x, x < lvl → ς1 x = ς2 x) →
-  lambda_expr_closed lvl e →
+Lemma subst_lambda_expr_scope ς1 ς2 scope e :
+  (∀ x, x < scope → ς1 x = ς2 x) →
+  lambda_expr_scope scope e →
   e.[ς1] = e.[ς2].
 Proof.
-  revert ς1 ς2 lvl. induction e as
+  revert ς1 ς2 scope. induction e as
     [ v
     | x
     | e1 IHe1 e2 IHe2
@@ -119,113 +119,113 @@ Proof.
     | e1 IHe1 e2 IHe2
     | e1 IHe1 e2 IHe2 e3 IHe3
     ];
-    intros ς1 ς2 lvl Hς Hclosed;
+    intros ς1 ς2 scope Hς Hscope;
     asimpl;
     try (f_equal; naive_solver).
   f_equal; first naive_solver.
   eapply IHe2; last naive_solver.
   intros x Hx. destruct x; first done. asimpl. f_equal. naive_solver lia.
 Qed.
-Lemma subst_lambda_expr_closed_0 ς1 ς2 e :
-  lambda_expr_closed 0 e →
+Lemma subst_lambda_expr_scope_0 ς1 ς2 e :
+  lambda_expr_scope 0 e →
   e.[ς1] = e.[ς2].
 Proof.
-  intros Hclosed.
-  eapply subst_lambda_expr_closed; last done.
+  intros Hscope.
+  eapply subst_lambda_expr_scope; last done.
   lia.
 Qed.
-Lemma subst_lambda_expr_closed_1 ς1 ς2 e :
+Lemma subst_lambda_expr_scope_1 ς1 ς2 e :
   ς1 0 = ς2 0 →
-  lambda_expr_closed 1 e →
+  lambda_expr_scope 1 e →
   e.[ς1] = e.[ς2].
 Proof.
-  intros Hς Hclosed.
-  eapply subst_lambda_expr_closed; last done.
+  intros Hς Hscope.
+  eapply subst_lambda_expr_scope; last done.
   setoid_rewrite Nat.lt_1_r. naive_solver.
 Qed.
-Lemma subst_lambda_expr_closed_1' ς1 ς2 v e :
-  lambda_expr_closed 1 e →
+Lemma subst_lambda_expr_scope_1' ς1 ς2 v e :
+  lambda_expr_scope 1 e →
   e.[v .: ς1] = e.[v .: ς2].
 Proof.
-  apply subst_lambda_expr_closed_1. done.
+  apply subst_lambda_expr_scope_1. done.
 Qed.
 
-Lemma subst_lambda_program_closed ς1 ς2 prog func e :
+Lemma subst_lambda_program_scope ς1 ς2 prog func e :
   ς1 0 = ς2 0 →
-  lambda_program_closed prog →
+  lambda_program_scope prog →
   prog !! func = Some e →
   e.[ς1] = e.[ς2].
 Proof.
   intros Hσ Hwf Hlookup.
-  eapply subst_lambda_expr_closed_1; first done.
+  eapply subst_lambda_expr_scope_1; first done.
   eapply map_Forall_lookup_1 in Hwf; naive_solver.
 Qed.
-Lemma subst_lambda_program_closed' ς1 ς2 v prog func e :
-  lambda_program_closed prog →
+Lemma subst_lambda_program_scope' ς1 ς2 v prog func e :
+  lambda_program_scope prog →
   prog !! func = Some e →
   e.[v .: ς1] = e.[v .: ς2].
 Proof.
-  apply subst_lambda_program_closed. done.
+  apply subst_lambda_program_scope. done.
 Qed.
 
-Lemma lambda_expr_closed_le lvl1 lvl2 e :
-  lvl1 ≤ lvl2 →
-  lambda_expr_closed lvl1 e →
-  lambda_expr_closed lvl2 e.
+Lemma lambda_expr_scope_le scope1 scope2 e :
+  scope1 ≤ scope2 →
+  lambda_expr_scope scope1 e →
+  lambda_expr_scope scope2 e.
 Proof.
-  revert lvl1 lvl2. elim e; try naive_solver lia.
-  intros e1 IH1 e2 IH2 lvl1 lvl2 Hlvl (Hclosed1 & Hclosed2).
+  revert scope1 scope2. elim e; try naive_solver lia.
+  intros e1 IH1 e2 IH2 scope1 scope2 Hscope (Hscope1 & Hscope2).
   split; first naive_solver. eapply IH2; last done. lia.
 Qed.
 
-Lemma lambda_expr_closed_upn_subst_lambda_val n v lvl e :
-  n < lvl →
-  lambda_expr_closed lvl e →
-  lambda_expr_closed (lvl - 1) e.[upn n (LambdaVal v .: ids)].
+Lemma lambda_expr_scope_upn_subst_lambda_val n v scope e :
+  n < scope →
+  lambda_expr_scope scope e →
+  lambda_expr_scope (scope - 1) e.[upn n (LambdaVal v .: ids)].
 Proof.
-  revert n lvl. induction e; intros n lvl; try naive_solver; simpl.
+  revert n scope. induction e; intros n scope; try naive_solver; simpl.
   - intros Hn Hx.
     destruct (Nat.lt_ge_cases x n) as [Hx' | (dx & ->)%Nat.le_sum].
     + rewrite upn_lt //=. lia.
     + rewrite upn_ge; first lia.
       rewrite Nat.sub_add'. destruct dx; first done. simpl. lia.
-  - intros Hn (Hclosed1 & Hclosed2). split; first naive_solver.
+  - intros Hn (Hscope1 & Hscope2). split; first naive_solver.
     rewrite fold_up_upn.
-    destruct lvl; first lia.
-    rewrite /= Nat.sub_0_r -(Nat.pred_succ (S lvl)) -Nat.sub_1_r.
+    destruct scope; first lia.
+    rewrite /= Nat.sub_0_r -(Nat.pred_succ (S scope)) -Nat.sub_1_r.
     auto with lia.
 Qed.
-Lemma lambda_expr_closed_subst_lambda_val lvl e v :
-  lambda_expr_closed lvl e →
-  lambda_expr_closed (lvl - 1) e.[LambdaVal v/].
+Lemma lambda_expr_scope_subst_lambda_val scope e v :
+  lambda_expr_scope scope e →
+  lambda_expr_scope (scope - 1) e.[LambdaVal v/].
 Proof.
-  destruct lvl.
-  - intros Hclosed%(lambda_expr_closed_le _ 1)%(lambda_expr_closed_upn_subst_lambda_val 0 v); naive_solver lia.
-  - apply (lambda_expr_closed_upn_subst_lambda_val 0). lia.
+  destruct scope.
+  - intros Hscope%(lambda_expr_scope_le _ 1)%(lambda_expr_scope_upn_subst_lambda_val 0 v); naive_solver lia.
+  - apply (lambda_expr_scope_upn_subst_lambda_val 0). lia.
 Qed.
 
-Lemma lambda_expr_closed_ren ξ n lvl e :
+Lemma lambda_expr_scope_ren ξ n scope e :
   (∀ x, ξ x ≤ x + n) →
-  lambda_expr_closed lvl e →
-  lambda_expr_closed (lvl + n) e.[ren ξ].
+  lambda_expr_scope scope e →
+  lambda_expr_scope (scope + n) e.[ren ξ].
 Proof.
-  revert lvl ξ n. elim e; try naive_solver lia.
-  - intros x lvl ξ n Hξ Hclosed.
+  revert scope ξ n. elim e; try naive_solver lia.
+  - intros x scope ξ n Hξ Hscope.
     eapply (Nat.le_lt_trans _ (x + n)); naive_solver lia.
-  - intros e1 IH1 e2 IH2 lvl ξ n Hξ (Hclosed1 & Hclosed2).
+  - intros e1 IH1 e2 IH2 scope ξ n Hξ (Hscope1 & Hscope2).
     split; first naive_solver.
     asimpl. rewrite -Nat.add_succ_l. apply IH2; last done.
     intros []; simpl; [lia | rewrite -Nat.succ_le_mono //].
 Qed.
-Lemma lambda_expr_closed_lift n lvl e :
-  lambda_expr_closed lvl e →
-  lambda_expr_closed (lvl + n) e.[ren (+n)].
+Lemma lambda_expr_scope_lift n scope e :
+  lambda_expr_scope scope e →
+  lambda_expr_scope (scope + n) e.[ren (+n)].
 Proof.
-  apply lambda_expr_closed_ren. naive_solver lia.
+  apply lambda_expr_scope_ren. naive_solver lia.
 Qed.
-Lemma lambda_expr_closed_lift1 lvl e :
-  lambda_expr_closed lvl e →
-  lambda_expr_closed (S lvl) e.[ren (+1)].
+Lemma lambda_expr_scope_lift1 scope e :
+  lambda_expr_scope scope e →
+  lambda_expr_scope (S scope) e.[ren (+1)].
 Proof.
-  rewrite -Nat.add_1_r. apply lambda_expr_closed_lift.
+  rewrite -Nat.add_1_r. apply lambda_expr_scope_lift.
 Qed.
