theories/tmc/properties.v
@@ -61,85 +61,85 @@ Section tmc.
     eauto using (proj2 tmc_subst).
   Qed.
 
-  Lemma lambda_expr_closed_tmc :
+  Lemma lambda_expr_scope_tmc :
     ( ∀ eₛ eₜ,
       tmc_dir ξ eₛ eₜ →
-      ∀ lvl,
-      lambda_expr_closed lvl eₛ →
-      lambda_expr_closed lvl eₜ
+      ∀ scope,
+      lambda_expr_scope scope eₛ →
+      lambda_expr_scope scope eₜ
     ) ∧ (
       ∀ dst idx eₛ eₜ,
       tmc_dps ξ dst idx eₛ eₜ →
-      ∀ lvl,
-      lambda_expr_closed lvl dst →
-      lambda_expr_closed lvl idx →
-      lambda_expr_closed lvl eₛ →
-      lambda_expr_closed lvl eₜ
+      ∀ scope,
+      lambda_expr_scope scope dst →
+      lambda_expr_scope scope idx →
+      lambda_expr_scope scope eₛ →
+      lambda_expr_scope scope eₜ
     ).
   Proof.
     apply tmc_ind; try naive_solver.
-    - intros * Hdir1 IH1 Hdps2 IH2 lvl (Hclosed1 & Hclosed2).
+    - intros * Hdir1 IH1 Hdps2 IH2 scope (Hscope1 & Hscope2).
       simpl. split_and!; try naive_solver lia.
       apply IH2; try naive_solver lia.
-      apply lambda_expr_closed_lift1. done.
-    - intros * Hdir2 IH2 Hdps1 IH1 lvl (Hclosed1 & Hclosed2).
+      apply lambda_expr_scope_lift1. done.
+    - intros * Hdir2 IH2 Hdps1 IH1 scope (Hscope1 & Hscope2).
       simpl. split_and!; try naive_solver lia.
       apply IH1; try naive_solver lia.
-      apply lambda_expr_closed_lift1. done.
-    - intros * Hdir1 IH1 Hdps2 IH2 lvl Hdst Hidx (Hclosed1 & Hclosed2).
+      apply lambda_expr_scope_lift1. done.
+    - intros * Hdir1 IH1 Hdps2 IH2 scope Hdst Hidx (Hscope1 & Hscope2).
       split; first auto.
-      apply IH2; try done; apply lambda_expr_closed_lift1; done.
-    - intros * Hξ Hdir IH -> lvl Hdst Hidx (_ & Hwf).
-      simpl. split_and!; [eauto using lambda_expr_closed_lift1.. | lia].
-    - intros * Hdir1 IH1 Hdps2 IH2 -> lvl Hdst Hidx (Hwf1 & Hwf2).
+      apply IH2; try done; apply lambda_expr_scope_lift1; done.
+    - intros * Hξ Hdir IH -> scope Hdst Hidx (_ & Hwf).
+      simpl. split_and!; [eauto using lambda_expr_scope_lift1.. | lia].
+    - intros * Hdir1 IH1 Hdps2 IH2 -> scope Hdst Hidx (Hwf1 & Hwf2).
       simpl. split_and!; try naive_solver lia.
-      + apply lambda_expr_closed_lift1. done.
-      + apply lambda_expr_closed_lift1. done.
-      + apply (lambda_expr_closed_le (S (S lvl))); first lia.
-        apply lambda_expr_closed_lift1, IH2; try naive_solver lia.
-        apply lambda_expr_closed_lift1. done.
-    - intros * Hdir2 IH2 Hdps1 IH1 -> lvl Hdst Hidx (Hwf1 & Hwf2).
+      + apply lambda_expr_scope_lift1. done.
+      + apply lambda_expr_scope_lift1. done.
+      + apply (lambda_expr_scope_le (S (S scope))); first lia.
+        apply lambda_expr_scope_lift1, IH2; try naive_solver lia.
+        apply lambda_expr_scope_lift1. done.
+    - intros * Hdir2 IH2 Hdps1 IH1 -> scope Hdst Hidx (Hwf1 & Hwf2).
       simpl. split_and!; try naive_solver lia.
-      + apply lambda_expr_closed_lift1. done.
-      + apply lambda_expr_closed_lift1. done.
-      + apply (lambda_expr_closed_le (S (S lvl))); first lia.
-        apply lambda_expr_closed_lift1, IH1; try naive_solver lia.
-        apply lambda_expr_closed_lift1. done.
+      + apply lambda_expr_scope_lift1. done.
+      + apply lambda_expr_scope_lift1. done.
+      + apply (lambda_expr_scope_le (S (S scope))); first lia.
+        apply lambda_expr_scope_lift1, IH1; try naive_solver lia.
+        apply lambda_expr_scope_lift1. done.
   Qed.
-  Lemma lambda_expr_closed_tmc_dir lvl eₛ eₜ :
+  Lemma lambda_expr_scope_tmc_dir scope eₛ eₜ :
     tmc_dir ξ eₛ eₜ →
-    lambda_expr_closed lvl eₛ →
-    lambda_expr_closed lvl eₜ.
+    lambda_expr_scope scope eₛ →
+    lambda_expr_scope scope eₜ.
   Proof.
-    eauto using (proj1 lambda_expr_closed_tmc).
+    eauto using (proj1 lambda_expr_scope_tmc).
   Qed.
-  Lemma lambda_expr_closed_tmc_dps lvl dst idx eₛ eₜ :
+  Lemma lambda_expr_scope_tmc_dps scope dst idx eₛ eₜ :
     tmc_dps ξ dst idx eₛ eₜ →
-    lambda_expr_closed lvl dst →
-    lambda_expr_closed lvl idx →
-    lambda_expr_closed lvl eₛ →
-    lambda_expr_closed lvl eₜ.
+    lambda_expr_scope scope dst →
+    lambda_expr_scope scope idx →
+    lambda_expr_scope scope eₛ →
+    lambda_expr_scope scope eₜ.
   Proof.
-    eauto using (proj2 lambda_expr_closed_tmc).
+    eauto using (proj2 lambda_expr_scope_tmc).
   Qed.
 End tmc.
 
 #[export] Hint Resolve tmc_dir_refl : tmc.
 
-Lemma lambda_program_closed_tmc progₛ progₜ :
+Lemma lambda_program_scope_tmc progₛ progₜ :
   tmc progₛ progₜ →
-  lambda_program_closed progₛ →
-  lambda_program_closed progₜ.
+  lambda_program_scope progₛ →
+  lambda_program_scope progₜ.
 Proof.
-  intros tmc. rewrite /lambda_program_closed !map_Forall_lookup => Hclosed func eₜ Hfuncₜ.
+  intros tmc. rewrite /lambda_program_scope !map_Forall_lookup => Hscope func eₜ Hfuncₜ.
   apply elem_of_dom_2 in Hfuncₜ as Hfuncₜ'. rewrite tmc.(tmc_dom) elem_of_union in Hfuncₜ'.
   destruct Hfuncₜ' as [Hfuncₛ%lookup_lookup_total_dom | (func_dir & Hξ)%elem_of_map_img].
   - edestruct tmc.(tmc_dirs) as (_eₜ & Hdir & Heq); first done.
-    eapply lambda_expr_closed_tmc_dir; last naive_solver.
+    eapply lambda_expr_scope_tmc_dir; last naive_solver.
     rewrite Heq in Hfuncₜ. naive_solver.
   - pose proof Hξ as Hfunc_dirₛ%elem_of_dom_2%(tmc.(tmc_ξ_dom))%lookup_lookup_total_dom.
     edestruct tmc.(tmc_dpss) as (eₜ' & Hdps & Heq); [done.. |].
     rewrite Hfuncₜ in Heq. injection Heq as ->.
-    repeat constructor. eapply lambda_expr_closed_tmc_dps; [naive_solver.. |].
-    apply (lambda_expr_closed_le 1); naive_solver lia.
+    repeat constructor. eapply lambda_expr_scope_tmc_dps; [naive_solver.. |].
+    apply (lambda_expr_scope_le 1); naive_solver lia.
 Qed.
