theories/tmc/soundness.v
@@ -282,15 +282,15 @@ Section sim_GS.
     SIM eₛ ≳ eₜ [[ tmc_protocol ]] {{# Φ }} -∗
     SIM eₛ ≳ eₜ {{# Φ }}.
   Proof.
-    intros (Hprogₛ_wf & Hprogₛ_closed).
-    eapply lambda_program_closed_tmc in Hprogₛ_closed as Hprogₜ_closed; last done.
+    intros (Hprogₛ_wf & Hprogₛ_scope).
+    eapply lambda_program_scope_tmc in Hprogₛ_scope as Hprogₜ_scope; last done.
     iApply sim_close_pure_head_step. clear eₛ eₜ. iIntros "!> %Ψ %eₛ %eₜ [Hprotocol | Hprotocol]".
     - iDestruct "Hprotocol" as "(%func & %vₛ & %vₜ & %Hfuncₛ & (-> & ->) & #Hv & HΨ)".
       simpl in Hfuncₛ. apply lookup_lookup_total_dom in Hfuncₛ. set (eₛ := _ !!! _) in Hfuncₛ.
       edestruct tmc.(tmc_dirs) as (eₜ & Hdir & Hfuncₜ); first done.
       iExists eₛ.[#vₛ/], eₜ.[#vₜ/]. iSplit; first auto with lambda_lang.
-      erewrite (subst_lambda_program_closed' ids inhabitant); last done; last done.
-      erewrite (subst_lambda_program_closed' ids inhabitant); last done; last done.
+      erewrite (subst_lambda_program_scope' ids inhabitant); last done; last done.
+      erewrite (subst_lambda_program_scope' ids inhabitant); last done; last done.
       iDestruct (tmc_dir_specification $! tmc_dir_post with "[//] [] [//] []") as "Hsim"; eauto.
       + iApply (bisubst_cons_well_formed with "Hv").
         iApply bisubst_inhabitant_well_formed.
@@ -302,11 +302,11 @@ Section sim_GS.
       iExists eₛ.[#vₛ/], _. iSplit; first auto with lambda_lang.
       do 4 sim_loadₜ. sim_pures.
       eapply (tmc_dps_subst _ (ids 0 .: #dst .: #idx .: ren (+1))) in Hdps; [| autosubst..].
-      erewrite (subst_lambda_program_closed' _ (ren (+1))) in Hdps; last done; last done. asimpl in Hdps.
+      erewrite (subst_lambda_program_scope' _ (ren (+1))) in Hdps; last done; last done. asimpl in Hdps.
       replace eₜ.[#vₜ, #dst, #idx, #l2, #l1/] with eₜ.[ids 0 .: #dst .: #idx .: ren (+1)].[#vₜ, #l2, #l1/] by autosubst.
-      erewrite (subst_lambda_program_closed' ids inhabitant); last done; last done.
-      erewrite (subst_lambda_expr_closed_1' (#l2 .: #l1 .: ids) inhabitant); last first.
-      { eapply lambda_expr_closed_tmc_dps; naive_solver. }
+      erewrite (subst_lambda_program_scope' ids inhabitant); last done; last done.
+      erewrite (subst_lambda_expr_scope_1' (#l2 .: #l1 .: ids) inhabitant); last first.
+      { eapply lambda_expr_scope_tmc_dps; naive_solver. }
       iDestruct (tmc_dps_specification $! (tmc_dps_post dst idx) with "Hdst [] [//] []") as "Hsim"; eauto.
       + iApply (bisubst_cons_well_formed with "Hv").
         iApply bisubst_inhabitant_well_formed.
